tests/lock.v
@@ -1,0 +1,9 @@
+From HB Require Import structures.
+
+HB.lock Definition foo := 3.
+
+Definition nat1 := nat.
+
+HB.lock Definition bar : nat1 := 3.
+
+HB.lock Definition baz n : nat := 3 + n.
